<?xml version="1.0"?>
<rdf:RDF xmlns="https://github.com/danCazacu/WTra#"
     xml:base="https://github.com/danCazacu/WTra"
     xmlns:owl="http://www.w3.org/2002/07/owl#"
     xmlns:rdf="http://www.w3.org/1999/02/22-rdf-syntax-ns#"
     xmlns:xml="http://www.w3.org/XML/1998/namespace"
     xmlns:xsd="http://www.w3.org/2001/XMLSchema#"
     xmlns:WTra="https://github.com/danCazacu/WTra#"
     xmlns:rdfs="http://www.w3.org/2000/01/rdf-schema#">
    <owl:Ontology rdf:about="https://github.com/danCazacu/WTra"/>
    


    <!-- 
    ///////////////////////////////////////////////////////////////////////////////////////
    //
    // Datatypes
    //
    ///////////////////////////////////////////////////////////////////////////////////////
     -->

    


    <!-- http://www.w3.org/2002/07/owl#intersectionOf -->

    <rdfs:Datatype rdf:about="http://www.w3.org/2002/07/owl#intersectionOf"/>
    


    <!-- http://www.w3.org/2002/07/owl#unionOf -->

    <rdfs:Datatype rdf:about="http://www.w3.org/2002/07/owl#unionOf"/>
    


    <!-- 
    ///////////////////////////////////////////////////////////////////////////////////////
    //
    // Object Properties
    //
    ///////////////////////////////////////////////////////////////////////////////////////
     -->

    


    <!-- https://github.com/danCazacu/WTra#applicableTo -->

    <owl:ObjectProperty rdf:about="https://github.com/danCazacu/WTra#applicableTo">
        <rdfs:domain rdf:resource="https://github.com/danCazacu/WTra#Traffic_Sign"/>
        <rdfs:range rdf:resource="https://github.com/danCazacu/WTra#Person"/>
    </owl:ObjectProperty>
    


    <!-- https://github.com/danCazacu/WTra#hasBackgroundColor -->

    <owl:ObjectProperty rdf:about="https://github.com/danCazacu/WTra#hasBackgroundColor">
        <rdfs:subPropertyOf rdf:resource="https://github.com/danCazacu/WTra#hasColor"/>
        <rdfs:domain rdf:resource="https://github.com/danCazacu/WTra#Traffic_Sign"/>
        <rdfs:range rdf:resource="https://github.com/danCazacu/WTra#Color"/>
    </owl:ObjectProperty>
    


    <!-- https://github.com/danCazacu/WTra#hasBorderColor -->

    <owl:ObjectProperty rdf:about="https://github.com/danCazacu/WTra#hasBorderColor">
        <rdfs:subPropertyOf rdf:resource="https://github.com/danCazacu/WTra#hasColor"/>
        <rdfs:domain rdf:resource="https://github.com/danCazacu/WTra#Traffic_Sign"/>
        <rdfs:range rdf:resource="https://github.com/danCazacu/WTra#Color"/>
    </owl:ObjectProperty>
    


    <!-- https://github.com/danCazacu/WTra#hasCode -->

    <owl:ObjectProperty rdf:about="https://github.com/danCazacu/WTra#hasCode">
        <owl:inverseOf rdf:resource="https://github.com/danCazacu/WTra#isCountry"/>
        <rdfs:domain rdf:resource="https://github.com/danCazacu/WTra#Country"/>
        <rdfs:range rdf:resource="https://github.com/danCazacu/WTra#Country_Code"/>
    </owl:ObjectProperty>
    


    <!-- https://github.com/danCazacu/WTra#hasColor -->

    <owl:ObjectProperty rdf:about="https://github.com/danCazacu/WTra#hasColor">
        <rdf:type rdf:resource="http://www.w3.org/2002/07/owl#FunctionalProperty"/>
        <rdfs:domain rdf:resource="https://github.com/danCazacu/WTra#Traffic_Sign"/>
        <rdfs:range rdf:resource="https://github.com/danCazacu/WTra#Color"/>
    </owl:ObjectProperty>
    


    <!-- https://github.com/danCazacu/WTra#hasForm -->

    <owl:ObjectProperty rdf:about="https://github.com/danCazacu/WTra#hasForm">
        <rdfs:subPropertyOf rdf:resource="http://www.w3.org/2002/07/owl#topObjectProperty"/>
        <rdf:type rdf:resource="http://www.w3.org/2002/07/owl#FunctionalProperty"/>
        <rdfs:domain rdf:resource="https://github.com/danCazacu/WTra#Traffic_Sign"/>
        <rdfs:range rdf:resource="https://github.com/danCazacu/WTra#Shape"/>
    </owl:ObjectProperty>
    


    <!-- https://github.com/danCazacu/WTra#hasNotSign -->

    <owl:ObjectProperty rdf:about="https://github.com/danCazacu/WTra#hasNotSign">
        <owl:inverseOf rdf:resource="https://github.com/danCazacu/WTra#hasSign"/>
        <rdf:type rdf:resource="http://www.w3.org/2002/07/owl#FunctionalProperty"/>
        <rdfs:domain rdf:resource="https://github.com/danCazacu/WTra#Country"/>
        <rdfs:range rdf:resource="https://github.com/danCazacu/WTra#Traffic_Sign"/>
    </owl:ObjectProperty>
    


    <!-- https://github.com/danCazacu/WTra#hasSign -->

    <owl:ObjectProperty rdf:about="https://github.com/danCazacu/WTra#hasSign">
        <rdfs:domain rdf:resource="https://github.com/danCazacu/WTra#Country"/>
        <rdfs:range rdf:resource="https://github.com/danCazacu/WTra#Traffic_Sign"/>
        <rdfs:range>
            <owl:Restriction>
                <owl:onProperty rdf:resource="http://www.w3.org/2002/07/owl#topDataProperty"/>
                <owl:minQualifiedCardinality rdf:datatype="http://www.w3.org/2001/XMLSchema#nonNegativeInteger">1</owl:minQualifiedCardinality>
                <owl:onDataRange rdf:resource="http://www.w3.org/2002/07/owl#unionOf"/>
            </owl:Restriction>
        </rdfs:range>
    </owl:ObjectProperty>
    


    <!-- https://github.com/danCazacu/WTra#isCountry -->

    <owl:ObjectProperty rdf:about="https://github.com/danCazacu/WTra#isCountry">
        <rdfs:subPropertyOf rdf:resource="http://www.w3.org/2002/07/owl#topObjectProperty"/>
        <rdf:type rdf:resource="http://www.w3.org/2002/07/owl#FunctionalProperty"/>
        <rdf:type rdf:resource="http://www.w3.org/2002/07/owl#InverseFunctionalProperty"/>
        <rdfs:domain rdf:resource="https://github.com/danCazacu/WTra#Country_Code"/>
        <rdfs:range rdf:resource="https://github.com/danCazacu/WTra#Country"/>
    </owl:ObjectProperty>
    


    <!-- 
    ///////////////////////////////////////////////////////////////////////////////////////
    //
    // Data properties
    //
    ///////////////////////////////////////////////////////////////////////////////////////
     -->

    


    <!-- https://github.com/danCazacu/WTra#hasImageLink -->

    <owl:DatatypeProperty rdf:about="https://github.com/danCazacu/WTra#hasImageLink">
        <rdfs:domain rdf:resource="https://github.com/danCazacu/WTra#Traffic_Sign"/>
        <rdfs:range rdf:resource="http://www.w3.org/2001/XMLSchema#string"/>
    </owl:DatatypeProperty>
    


    <!-- https://github.com/danCazacu/WTra#hasLegalRegulations -->

    <owl:DatatypeProperty rdf:about="https://github.com/danCazacu/WTra#hasLegalRegulations">
        <rdfs:domain rdf:resource="https://github.com/danCazacu/WTra#Traffic_Sign"/>
    </owl:DatatypeProperty>
    


    <!-- 
    ///////////////////////////////////////////////////////////////////////////////////////
    //
    // Classes
    //
    ///////////////////////////////////////////////////////////////////////////////////////
     -->

    


    <!-- https://github.com/danCazacu/WTra#Color -->

    <owl:Class rdf:about="https://github.com/danCazacu/WTra#Color"/>
    


    <!-- https://github.com/danCazacu/WTra#Country -->

    <owl:Class rdf:about="https://github.com/danCazacu/WTra#Country">
        <owl:disjointWith rdf:resource="https://github.com/danCazacu/WTra#Traffic_Sign"/>
    </owl:Class>
    


    <!-- https://github.com/danCazacu/WTra#Country_Code -->

    <owl:Class rdf:about="https://github.com/danCazacu/WTra#Country_Code"/>
    


    <!-- https://github.com/danCazacu/WTra#Information_Sign -->

    <owl:Class rdf:about="https://github.com/danCazacu/WTra#Information_Sign">
        <rdfs:subClassOf rdf:resource="https://github.com/danCazacu/WTra#Traffic_Sign"/>
        <rdfs:comment>The information signs give you more information about the start (and end) of a kind of traffic situation.</rdfs:comment>
        <rdfs:label>Information Sign</rdfs:label>
    </owl:Class>
    


    <!-- https://github.com/danCazacu/WTra#Mandatory_Sign -->

    <owl:Class rdf:about="https://github.com/danCazacu/WTra#Mandatory_Sign">
        <rdfs:subClassOf rdf:resource="https://github.com/danCazacu/WTra#Traffic_Sign"/>
        <rdfs:comment>The mandatory signs impose an obligation/command that road users must comply with.</rdfs:comment>
        <rdfs:label>Mandatory Sign</rdfs:label>
    </owl:Class>
    


    <!-- https://github.com/danCazacu/WTra#Person -->

    <owl:Class rdf:about="https://github.com/danCazacu/WTra#Person"/>
    


    <!-- https://github.com/danCazacu/WTra#Priority_Sign -->

    <owl:Class rdf:about="https://github.com/danCazacu/WTra#Priority_Sign">
        <rdfs:subClassOf rdf:resource="https://github.com/danCazacu/WTra#Traffic_Sign"/>
        <rdfs:comment>The priority signs have an influence on the priority rules. They indicate who has priority and who should give priority.</rdfs:comment>
        <rdfs:label>Priority Sign</rdfs:label>
    </owl:Class>
    


    <!-- https://github.com/danCazacu/WTra#Prohibitory_Sign -->

    <owl:Class rdf:about="https://github.com/danCazacu/WTra#Prohibitory_Sign">
        <rdfs:subClassOf rdf:resource="https://github.com/danCazacu/WTra#Traffic_Sign"/>
        <rdfs:comment>The prohibition signs forbid a certain action. They indicate certain actions that road users are not allowed to do.</rdfs:comment>
        <rdfs:label>Prohibitory Sign</rdfs:label>
    </owl:Class>
    


    <!-- https://github.com/danCazacu/WTra#Road_Sign -->

    <owl:Class rdf:about="https://github.com/danCazacu/WTra#Road_Sign">
        <owl:equivalentClass rdf:resource="https://github.com/danCazacu/WTra#Traffic_Sign"/>
        <rdfs:subClassOf rdf:resource="https://github.com/danCazacu/WTra#Signs"/>
    </owl:Class>
    


    <!-- https://github.com/danCazacu/WTra#Safety_Sign -->

    <owl:Class rdf:about="https://github.com/danCazacu/WTra#Safety_Sign">
        <rdfs:subClassOf rdf:resource="https://github.com/danCazacu/WTra#Signs"/>
        <rdfs:comment>The safety signs are often used in companies or factories to provide information about safety.</rdfs:comment>
    </owl:Class>
    


    <!-- https://github.com/danCazacu/WTra#Shape -->

    <owl:Class rdf:about="https://github.com/danCazacu/WTra#Shape"/>
    


    <!-- https://github.com/danCazacu/WTra#Signs -->

    <owl:Class rdf:about="https://github.com/danCazacu/WTra#Signs"/>
    


    <!-- https://github.com/danCazacu/WTra#Traffic_Sign -->

    <owl:Class rdf:about="https://github.com/danCazacu/WTra#Traffic_Sign">
        <rdfs:subClassOf rdf:resource="https://github.com/danCazacu/WTra#Signs"/>
        <rdfs:comment>The traffic signs are located on the side or top of the road. They give directions on how we should behave on the road, so that the traffic can proceed safely and smoothly. Everyone must know the traffic signs!</rdfs:comment>
    </owl:Class>
    


    <!-- https://github.com/danCazacu/WTra#Warning_Sign -->

    <owl:Class rdf:about="https://github.com/danCazacu/WTra#Warning_Sign">
        <rdfs:subClassOf rdf:resource="https://github.com/danCazacu/WTra#Traffic_Sign"/>
        <rdfs:comment>The warning signs are placed to warn road users of a potentially dangerous traffic situation.</rdfs:comment>
        <rdfs:label>Warning Sign</rdfs:label>
    </owl:Class>
    


    <!-- 
    ///////////////////////////////////////////////////////////////////////////////////////
    //
    // Individuals
    //
    ///////////////////////////////////////////////////////////////////////////////////////
     -->

    


    <!-- https://github.com/danCazacu/WTra#a -->

    <owl:NamedIndividual rdf:about="https://github.com/danCazacu/WTra#a">
        <rdf:type rdf:resource="https://github.com/danCazacu/WTra#Country_Code"/>
    </owl:NamedIndividual>
    


    <!-- https://github.com/danCazacu/WTra#begin_of_a_priority_road -->

    <owl:NamedIndividual rdf:about="https://github.com/danCazacu/WTra#begin_of_a_priority_road">
        <rdf:type rdf:resource="https://github.com/danCazacu/WTra#Information_Sign"/>
        <rdf:type rdf:resource="https://github.com/danCazacu/WTra#Priority_Sign"/>
        <applicableTo rdf:resource="https://github.com/danCazacu/WTra#driver"/>
        <hasBackgroundColor rdf:resource="https://github.com/danCazacu/WTra#yellow"/>
        <hasBorderColor rdf:resource="https://github.com/danCazacu/WTra#white"/>
        <hasForm rdf:resource="https://github.com/danCazacu/WTra#diamond"/>
        <hasImageLink>https://traffic-rules.com/img/europe/ro/signs/information/information-priority-road.png</hasImageLink>
        <hasLegalRegulations>Priority road (priority at all following intersections up to an end-of-priority-road, yield or stop sign). In some countries, the meaning was changed to the next intersection only.</hasLegalRegulations>
        <rdfs:comment>This traffic sign indicates the begin of a priority road. You have priority at all following crossroads until the end of the priority road.</rdfs:comment>
    </owl:NamedIndividual>
    


    <!-- https://github.com/danCazacu/WTra#black -->

    <owl:NamedIndividual rdf:about="https://github.com/danCazacu/WTra#black">
        <rdf:type rdf:resource="https://github.com/danCazacu/WTra#Color"/>
    </owl:NamedIndividual>
    


    <!-- https://github.com/danCazacu/WTra#blue -->

    <owl:NamedIndividual rdf:about="https://github.com/danCazacu/WTra#blue">
        <rdf:type rdf:resource="https://github.com/danCazacu/WTra#Color"/>
    </owl:NamedIndividual>
    


    <!-- https://github.com/danCazacu/WTra#ch -->

    <owl:NamedIndividual rdf:about="https://github.com/danCazacu/WTra#ch">
        <rdf:type rdf:resource="https://github.com/danCazacu/WTra#Country_Code"/>
    </owl:NamedIndividual>
    


    <!-- https://github.com/danCazacu/WTra#circle -->

    <owl:NamedIndividual rdf:about="https://github.com/danCazacu/WTra#circle">
        <rdf:type rdf:resource="https://github.com/danCazacu/WTra#Shape"/>
    </owl:NamedIndividual>
    


    <!-- https://github.com/danCazacu/WTra#crossing_for_pedestrians -->

    <owl:NamedIndividual rdf:about="https://github.com/danCazacu/WTra#crossing_for_pedestrians">
        <rdf:type rdf:resource="https://github.com/danCazacu/WTra#Information_Sign"/>
        <applicableTo rdf:resource="https://github.com/danCazacu/WTra#driver"/>
        <applicableTo rdf:resource="https://github.com/danCazacu/WTra#pedestrian"/>
        <hasBackgroundColor rdf:resource="https://github.com/danCazacu/WTra#blue"/>
        <hasBorderColor rdf:resource="https://github.com/danCazacu/WTra#white"/>
        <hasForm rdf:resource="https://github.com/danCazacu/WTra#square"/>
        <hasImageLink>https://traffic-rules.com/img/europe/gr/signs/information/information-crossing-pedestrian.png</hasImageLink>
        <hasLegalRegulations>Pedestrian crossings allow people to cross the road safely. These crossings are usually marked by white stripes on the road and are also known as zebra crossings.

Some pedestrian crossings have zig zag lines marked on the road before the crossing. Take extra care when you see a zig zag line on the road as this means you are approaching a crossing which you may not be able to see because of a curve, crest or dip in the road.

Do not overtake any vehicle that is stopping or has stopped at a crossing.</hasLegalRegulations>
        <rdfs:comment>This traffic sign indicates a crossing for pedestrians.</rdfs:comment>
    </owl:NamedIndividual>
    


    <!-- https://github.com/danCazacu/WTra#cz -->

    <owl:NamedIndividual rdf:about="https://github.com/danCazacu/WTra#cz">
        <rdf:type rdf:resource="https://github.com/danCazacu/WTra#Country_Code"/>
    </owl:NamedIndividual>
    


    <!-- https://github.com/danCazacu/WTra#d -->

    <owl:NamedIndividual rdf:about="https://github.com/danCazacu/WTra#d">
        <rdf:type rdf:resource="https://github.com/danCazacu/WTra#Country_Code"/>
        <isCountry rdf:resource="https://github.com/danCazacu/WTra#germany"/>
    </owl:NamedIndividual>
    


    <!-- https://github.com/danCazacu/WTra#diamond -->

    <owl:NamedIndividual rdf:about="https://github.com/danCazacu/WTra#diamond">
        <rdf:type rdf:resource="https://github.com/danCazacu/WTra#Shape"/>
    </owl:NamedIndividual>
    


    <!-- https://github.com/danCazacu/WTra#driver -->

    <owl:NamedIndividual rdf:about="https://github.com/danCazacu/WTra#driver">
        <rdf:type rdf:resource="https://github.com/danCazacu/WTra#Person"/>
    </owl:NamedIndividual>
    


    <!-- https://github.com/danCazacu/WTra#end_of_the_priority_road_one_3_lines -->

    <owl:NamedIndividual rdf:about="https://github.com/danCazacu/WTra#end_of_the_priority_road_one_3_lines">
        <rdf:type rdf:resource="https://github.com/danCazacu/WTra#Information_Sign"/>
        <rdf:type rdf:resource="https://github.com/danCazacu/WTra#Priority_Sign"/>
        <owl:sameAs rdf:resource="https://github.com/danCazacu/WTra#end_of_the_priority_road_one_line"/>
        <applicableTo rdf:resource="https://github.com/danCazacu/WTra#driver"/>
        <hasBackgroundColor rdf:resource="https://github.com/danCazacu/WTra#yellow"/>
        <hasBorderColor rdf:resource="https://github.com/danCazacu/WTra#white"/>
        <hasForm rdf:resource="https://github.com/danCazacu/WTra#diamond"/>
        <hasImageLink>https://traffic-rules.com/img/europe/de/signs/information/information-priority-road_end.png</hasImageLink>
        <hasLegalRegulations>End of priority road (priority to the right applies at uncontrolled intersections)</hasLegalRegulations>
        <rdfs:comment>This traffic sign indicates the end of the priority road. You have no longer priority at the following crossroads.</rdfs:comment>
    </owl:NamedIndividual>
    


    <!-- https://github.com/danCazacu/WTra#end_of_the_priority_road_one_line -->

    <owl:NamedIndividual rdf:about="https://github.com/danCazacu/WTra#end_of_the_priority_road_one_line">
        <rdf:type rdf:resource="https://github.com/danCazacu/WTra#Information_Sign"/>
        <rdf:type rdf:resource="https://github.com/danCazacu/WTra#Priority_Sign"/>
        <applicableTo rdf:resource="https://github.com/danCazacu/WTra#driver"/>
        <hasBackgroundColor rdf:resource="https://github.com/danCazacu/WTra#yellow"/>
        <hasBorderColor rdf:resource="https://github.com/danCazacu/WTra#white"/>
        <hasForm rdf:resource="https://github.com/danCazacu/WTra#diamond"/>
        <hasImageLink>https://traffic-rules.com/img/europe/ro/signs/information/information-priority-road_end.png</hasImageLink>
        <hasLegalRegulations>End of priority road (priority to the right applies at uncontrolled intersections)</hasLegalRegulations>
        <rdfs:comment>This traffic sign indicates the end of the priority road. You have no longer priority at the following crossroads.</rdfs:comment>
    </owl:NamedIndividual>
    


    <!-- https://github.com/danCazacu/WTra#end_of_the_speed_limit_3_lines -->

    <owl:NamedIndividual rdf:about="https://github.com/danCazacu/WTra#end_of_the_speed_limit_3_lines">
        <rdf:type rdf:resource="https://github.com/danCazacu/WTra#Prohibitory_Sign"/>
        <owl:sameAs rdf:resource="https://github.com/danCazacu/WTra#end_of_the_speed_limit_one_line"/>
        <applicableTo rdf:resource="https://github.com/danCazacu/WTra#driver"/>
        <hasBackgroundColor rdf:resource="https://github.com/danCazacu/WTra#white"/>
        <hasBorderColor rdf:resource="https://github.com/danCazacu/WTra#black"/>
        <hasForm rdf:resource="https://github.com/danCazacu/WTra#circle"/>
        <hasImageLink>https://traffic-rules.com/img/europe/fi/signs/prohibitory/prohibited-action-speed_end.png</hasImageLink>
        <hasLegalRegulations>The traffic sign indicates the end of the speed limit. From now one the driver can pass the limit, but respecting though the limit for the area were he is driving (e.g.: expressway )</hasLegalRegulations>
        <rdfs:comment>This traffic sign indicates the end of the speed limit.</rdfs:comment>
    </owl:NamedIndividual>
    


    <!-- https://github.com/danCazacu/WTra#end_of_the_speed_limit_one_line -->

    <owl:NamedIndividual rdf:about="https://github.com/danCazacu/WTra#end_of_the_speed_limit_one_line">
        <rdf:type rdf:resource="https://github.com/danCazacu/WTra#Prohibitory_Sign"/>
        <applicableTo rdf:resource="https://github.com/danCazacu/WTra#driver"/>
        <hasBackgroundColor rdf:resource="https://github.com/danCazacu/WTra#white"/>
        <hasBorderColor rdf:resource="https://github.com/danCazacu/WTra#black"/>
        <hasForm rdf:resource="https://github.com/danCazacu/WTra#circle"/>
        <hasImageLink>https://traffic-rules.com/img/europe/ro/signs/prohibitory/prohibited-action-speed_end.png</hasImageLink>
        <hasLegalRegulations>The traffic sign indicates the end of the speed limit. From now one the driver can pass the limit, but respecting though the limit for the area were he is driving (e.g.: expressway )</hasLegalRegulations>
        <rdfs:comment>This traffic sign indicates the end of the speed limit.</rdfs:comment>
    </owl:NamedIndividual>
    


    <!-- https://github.com/danCazacu/WTra#f -->

    <owl:NamedIndividual rdf:about="https://github.com/danCazacu/WTra#f">
        <rdf:type rdf:resource="https://github.com/danCazacu/WTra#Country_Code"/>
    </owl:NamedIndividual>
    


    <!-- https://github.com/danCazacu/WTra#fin -->

    <owl:NamedIndividual rdf:about="https://github.com/danCazacu/WTra#fin">
        <rdf:type rdf:resource="https://github.com/danCazacu/WTra#Country_Code"/>
    </owl:NamedIndividual>
    


    <!-- https://github.com/danCazacu/WTra#finland -->

    <owl:NamedIndividual rdf:about="https://github.com/danCazacu/WTra#finland">
        <rdf:type rdf:resource="https://github.com/danCazacu/WTra#Country"/>
        <hasCode rdf:resource="https://github.com/danCazacu/WTra#fin"/>
        <hasSign rdf:resource="https://github.com/danCazacu/WTra#begin_of_a_priority_road"/>
        <hasSign rdf:resource="https://github.com/danCazacu/WTra#crossing_for_pedestrians"/>
        <hasSign rdf:resource="https://github.com/danCazacu/WTra#end_of_the_priority_road_one_3_lines"/>
        <hasSign rdf:resource="https://github.com/danCazacu/WTra#end_of_the_speed_limit_3_lines"/>
        <hasSign rdf:resource="https://github.com/danCazacu/WTra#give_way_to_all_drivers_red_yellow"/>
        <hasSign rdf:resource="https://github.com/danCazacu/WTra#mandatory_right"/>
        <hasSign rdf:resource="https://github.com/danCazacu/WTra#mandatory_shared_path_for_pedestrians_and_cyclists"/>
        <hasSign rdf:resource="https://github.com/danCazacu/WTra#maximum_speed_limit_red_yellow"/>
        <hasSign rdf:resource="https://github.com/danCazacu/WTra#no_motor_vehicles_red_yellow"/>
        <hasSign rdf:resource="https://github.com/danCazacu/WTra#other_danger_red_yellow"/>
        <hasSign rdf:resource="https://github.com/danCazacu/WTra#pedestrians_prohibited_red_yellow"/>
        <hasSign rdf:resource="https://github.com/danCazacu/WTra#stop_and_give_way_to_all_drivers"/>
        <hasSign rdf:resource="https://github.com/danCazacu/WTra#turning_left_prohibited_red_yellow"/>
        <hasSign rdf:resource="https://github.com/danCazacu/WTra#turning_right_mandatory"/>
        <hasSign rdf:resource="https://github.com/danCazacu/WTra#turning_right_prohibited_red_yellow"/>
        <hasSign rdf:resource="https://github.com/danCazacu/WTra#warning_for_a_crossing_for_pedestrians_red_yellow"/>
        <hasSign rdf:resource="https://github.com/danCazacu/WTra#warning_for_a_traffic_light_red_yellow"/>
        <hasSign rdf:resource="https://github.com/danCazacu/WTra#warning_for_children_red_yellow"/>
        <hasSign rdf:resource="https://github.com/danCazacu/WTra#warning_for_traffic_jams_red_black"/>
    </owl:NamedIndividual>
    


    <!-- https://github.com/danCazacu/WTra#gb -->

    <owl:NamedIndividual rdf:about="https://github.com/danCazacu/WTra#gb">
        <rdf:type rdf:resource="https://github.com/danCazacu/WTra#Country_Code"/>
        <isCountry rdf:resource="https://github.com/danCazacu/WTra#united_kindom"/>
    </owl:NamedIndividual>
    


    <!-- https://github.com/danCazacu/WTra#general_warning_sign -->

    <owl:NamedIndividual rdf:about="https://github.com/danCazacu/WTra#general_warning_sign">
        <rdf:type rdf:resource="https://github.com/danCazacu/WTra#Safety_Sign"/>
        <hasImageLink>https://traffic-rules.com/img/international/safety-signs/warning.png</hasImageLink>
    </owl:NamedIndividual>
    


    <!-- https://github.com/danCazacu/WTra#germany -->

    <owl:NamedIndividual rdf:about="https://github.com/danCazacu/WTra#germany">
        <rdf:type rdf:resource="https://github.com/danCazacu/WTra#Country"/>
        <hasCode rdf:resource="https://github.com/danCazacu/WTra#d"/>
        <hasNotSign rdf:resource="https://github.com/danCazacu/WTra#other_danger_red_white"/>
        <hasNotSign rdf:resource="https://github.com/danCazacu/WTra#other_danger_red_yellow"/>
        <hasSign rdf:resource="https://github.com/danCazacu/WTra#begin_of_a_priority_road"/>
        <hasSign rdf:resource="https://github.com/danCazacu/WTra#crossing_for_pedestrians"/>
        <hasSign rdf:resource="https://github.com/danCazacu/WTra#end_of_the_priority_road_one_3_lines"/>
        <hasSign rdf:resource="https://github.com/danCazacu/WTra#end_of_the_speed_limit_one_line"/>
        <hasSign rdf:resource="https://github.com/danCazacu/WTra#give_way_to_all_drivers_red_white"/>
        <hasSign rdf:resource="https://github.com/danCazacu/WTra#mandatory_right"/>
        <hasSign rdf:resource="https://github.com/danCazacu/WTra#mandatory_shared_path_for_pedestrians_and_cyclists"/>
        <hasSign rdf:resource="https://github.com/danCazacu/WTra#maximum_speed_limit_red_white"/>
        <hasSign rdf:resource="https://github.com/danCazacu/WTra#minimum_speed_limit"/>
        <hasSign rdf:resource="https://github.com/danCazacu/WTra#no_motor_vehicles_red_white"/>
        <hasSign rdf:resource="https://github.com/danCazacu/WTra#pedestrians_prohibited_red_white"/>
        <hasSign rdf:resource="https://github.com/danCazacu/WTra#stop_and_give_way_to_all_drivers"/>
        <hasSign rdf:resource="https://github.com/danCazacu/WTra#turning_left_prohibited_red_white"/>
        <hasSign rdf:resource="https://github.com/danCazacu/WTra#turning_right_mandatory"/>
        <hasSign rdf:resource="https://github.com/danCazacu/WTra#turning_right_prohibited_red_white"/>
        <hasSign rdf:resource="https://github.com/danCazacu/WTra#warning_for_a_crossing_for_pedestrians_red_white"/>
        <hasSign rdf:resource="https://github.com/danCazacu/WTra#warning_for_a_traffic_light_red_white"/>
        <hasSign rdf:resource="https://github.com/danCazacu/WTra#warning_for_children_red_white"/>
        <hasSign rdf:resource="https://github.com/danCazacu/WTra#warning_for_traffic_jams_red_white"/>
        <rdfs:seeAlso>https://www.wikiwand.com/en/Germany</rdfs:seeAlso>
    </owl:NamedIndividual>
    


    <!-- https://github.com/danCazacu/WTra#give_way_to_all_drivers_red_white -->

    <owl:NamedIndividual rdf:about="https://github.com/danCazacu/WTra#give_way_to_all_drivers_red_white">
        <rdf:type rdf:resource="https://github.com/danCazacu/WTra#Priority_Sign"/>
        <rdf:type rdf:resource="https://github.com/danCazacu/WTra#Warning_Sign"/>
        <owl:sameAs rdf:resource="https://github.com/danCazacu/WTra#give_way_to_all_drivers_red_yellow"/>
        <applicableTo rdf:resource="https://github.com/danCazacu/WTra#driver"/>
        <hasBackgroundColor rdf:resource="https://github.com/danCazacu/WTra#white"/>
        <hasBorderColor rdf:resource="https://github.com/danCazacu/WTra#red"/>
        <hasForm rdf:resource="https://github.com/danCazacu/WTra#triangle"/>
        <hasImageLink>https://traffic-rules.com/img/europe/ro/signs/warning/warning-crossroad-give-way.png</hasImageLink>
        <hasLegalRegulations>This traffic sign means that the driver is not allowed to enter the crossroad unless the road is clear. He is not forced to stop the car.</hasLegalRegulations>
        <rdfs:comment>This traffic sign warns for a crossroad and indicates who has priority. This traffic sign means that the driver is not allowed to enter the crossroad unless the road is clear.</rdfs:comment>
    </owl:NamedIndividual>
    


    <!-- https://github.com/danCazacu/WTra#give_way_to_all_drivers_red_yellow -->

    <owl:NamedIndividual rdf:about="https://github.com/danCazacu/WTra#give_way_to_all_drivers_red_yellow">
        <rdf:type rdf:resource="https://github.com/danCazacu/WTra#Priority_Sign"/>
        <rdf:type rdf:resource="https://github.com/danCazacu/WTra#Warning_Sign"/>
        <applicableTo rdf:resource="https://github.com/danCazacu/WTra#driver"/>
        <hasBackgroundColor rdf:resource="https://github.com/danCazacu/WTra#yellow"/>
        <hasBorderColor rdf:resource="https://github.com/danCazacu/WTra#red"/>
        <hasForm rdf:resource="https://github.com/danCazacu/WTra#triangle"/>
        <hasImageLink>https://traffic-rules.com/img/europe/gr/signs/warning/warning-crossroad-give-way.png</hasImageLink>
        <hasLegalRegulations>This traffic sign means that the driver is not allowed to enter the crossroad unless the road is clear. The driver is not forced to stop the car.</hasLegalRegulations>
        <rdfs:comment>This traffic sign warns for a crossroad and indicates who has priority. This traffic sign means that the driver is not allowed to enter the crossroad unless the road is clear.</rdfs:comment>
    </owl:NamedIndividual>
    


    <!-- https://github.com/danCazacu/WTra#gr -->

    <owl:NamedIndividual rdf:about="https://github.com/danCazacu/WTra#gr">
        <rdf:type rdf:resource="https://github.com/danCazacu/WTra#Country_Code"/>
    </owl:NamedIndividual>
    


    <!-- https://github.com/danCazacu/WTra#green -->

    <owl:NamedIndividual rdf:about="https://github.com/danCazacu/WTra#green">
        <rdf:type rdf:resource="https://github.com/danCazacu/WTra#Color"/>
    </owl:NamedIndividual>
    


    <!-- https://github.com/danCazacu/WTra#grey -->

    <owl:NamedIndividual rdf:about="https://github.com/danCazacu/WTra#grey">
        <rdf:type rdf:resource="https://github.com/danCazacu/WTra#Color"/>
    </owl:NamedIndividual>
    


    <!-- https://github.com/danCazacu/WTra#hexagon -->

    <owl:NamedIndividual rdf:about="https://github.com/danCazacu/WTra#hexagon">
        <rdf:type rdf:resource="https://github.com/danCazacu/WTra#Shape"/>
    </owl:NamedIndividual>
    


    <!-- https://github.com/danCazacu/WTra#i -->

    <owl:NamedIndividual rdf:about="https://github.com/danCazacu/WTra#i">
        <rdf:type rdf:resource="https://github.com/danCazacu/WTra#Country_Code"/>
        <isCountry rdf:resource="https://github.com/danCazacu/WTra#italy"/>
    </owl:NamedIndividual>
    


    <!-- https://github.com/danCazacu/WTra#ireland -->

    <owl:NamedIndividual rdf:about="https://github.com/danCazacu/WTra#ireland">
        <rdf:type rdf:resource="https://github.com/danCazacu/WTra#Country"/>
        <hasCode rdf:resource="https://github.com/danCazacu/WTra#irl"/>
        <hasNotSign rdf:resource="https://github.com/danCazacu/WTra#begin_of_a_priority_road"/>
        <hasNotSign rdf:resource="https://github.com/danCazacu/WTra#end_of_the_priority_road_one_3_lines"/>
        <hasNotSign rdf:resource="https://github.com/danCazacu/WTra#end_of_the_priority_road_one_line"/>
        <hasNotSign rdf:resource="https://github.com/danCazacu/WTra#minimum_speed_limit"/>
        <hasNotSign rdf:resource="https://github.com/danCazacu/WTra#other_danger_red_white"/>
        <hasSign rdf:resource="https://github.com/danCazacu/WTra#crossing_for_pedestrians"/>
        <hasSign rdf:resource="https://github.com/danCazacu/WTra#end_of_the_speed_limit_one_line"/>
        <hasSign rdf:resource="https://github.com/danCazacu/WTra#give_way_to_all_drivers_red_white"/>
        <hasSign rdf:resource="https://github.com/danCazacu/WTra#mandatory_right"/>
        <hasSign rdf:resource="https://github.com/danCazacu/WTra#mandatory_shared_path_for_pedestrians_and_cyclists"/>
        <hasSign rdf:resource="https://github.com/danCazacu/WTra#maximum_speed_limit_red_white"/>
        <hasSign rdf:resource="https://github.com/danCazacu/WTra#pedestrians_prohibited_red_white"/>
        <hasSign rdf:resource="https://github.com/danCazacu/WTra#stop_and_give_way_to_all_drivers"/>
        <hasSign rdf:resource="https://github.com/danCazacu/WTra#turning_left_prohibited_red_white"/>
        <hasSign rdf:resource="https://github.com/danCazacu/WTra#turning_right_mandatory"/>
        <hasSign rdf:resource="https://github.com/danCazacu/WTra#turning_right_prohibited_red_white"/>
        <hasSign rdf:resource="https://github.com/danCazacu/WTra#warning_for_a_crossing_for_pedestrians_red_white"/>
        <hasSign rdf:resource="https://github.com/danCazacu/WTra#warning_for_a_traffic_light_diamond"/>
        <hasSign rdf:resource="https://github.com/danCazacu/WTra#warning_for_children_red_white"/>
        <hasSign rdf:resource="https://github.com/danCazacu/WTra#warning_for_traffic_jams_red_yellow"/>
        <rdfs:comment>Road signs in Ireland do not differ greatly from those used elsewhere in Europe, but there are some differences between those used in the Republic of Ireland and those used in Northern Ireland, including different systems of units used in each jurisdiction.</rdfs:comment>
        <rdfs:seeAlso>https://www.wikiwand.com/en/Republic_of_Ireland</rdfs:seeAlso>
    </owl:NamedIndividual>
    


    <!-- https://github.com/danCazacu/WTra#irl -->

    <owl:NamedIndividual rdf:about="https://github.com/danCazacu/WTra#irl">
        <rdf:type rdf:resource="https://github.com/danCazacu/WTra#Country_Code"/>
        <isCountry rdf:resource="https://github.com/danCazacu/WTra#ireland"/>
    </owl:NamedIndividual>
    


    <!-- https://github.com/danCazacu/WTra#italy -->

    <owl:NamedIndividual rdf:about="https://github.com/danCazacu/WTra#italy">
        <rdf:type rdf:resource="https://github.com/danCazacu/WTra#Country"/>
        <hasCode rdf:resource="https://github.com/danCazacu/WTra#i"/>
        <hasNotSign rdf:resource="https://github.com/danCazacu/WTra#no_motor_vehicles_red_white"/>
        <hasNotSign rdf:resource="https://github.com/danCazacu/WTra#no_motor_vehicles_red_yellow"/>
        <hasSign rdf:resource="https://github.com/danCazacu/WTra#begin_of_a_priority_road"/>
        <hasSign rdf:resource="https://github.com/danCazacu/WTra#crossing_for_pedestrians"/>
        <hasSign rdf:resource="https://github.com/danCazacu/WTra#end_of_the_priority_road_one_line"/>
        <hasSign rdf:resource="https://github.com/danCazacu/WTra#end_of_the_speed_limit_one_line"/>
        <hasSign rdf:resource="https://github.com/danCazacu/WTra#give_way_to_all_drivers_red_white"/>
        <hasSign rdf:resource="https://github.com/danCazacu/WTra#mandatory_right"/>
        <hasSign rdf:resource="https://github.com/danCazacu/WTra#mandatory_shared_path_for_pedestrians_and_cyclists"/>
        <hasSign rdf:resource="https://github.com/danCazacu/WTra#maximum_speed_limit_red_white"/>
        <hasSign rdf:resource="https://github.com/danCazacu/WTra#minimum_speed_limit"/>
        <hasSign rdf:resource="https://github.com/danCazacu/WTra#other_danger_red_yellow"/>
        <hasSign rdf:resource="https://github.com/danCazacu/WTra#pedestrians_prohibited_red_white"/>
        <hasSign rdf:resource="https://github.com/danCazacu/WTra#stop_and_give_way_to_all_drivers"/>
        <hasSign rdf:resource="https://github.com/danCazacu/WTra#turning_left_prohibited_red_white"/>
        <hasSign rdf:resource="https://github.com/danCazacu/WTra#turning_right_mandatory"/>
        <hasSign rdf:resource="https://github.com/danCazacu/WTra#turning_right_prohibited_red_white"/>
        <hasSign rdf:resource="https://github.com/danCazacu/WTra#warning_for_a_crossing_for_pedestrians_red_white"/>
        <hasSign rdf:resource="https://github.com/danCazacu/WTra#warning_for_a_traffic_light_red_white"/>
        <hasSign rdf:resource="https://github.com/danCazacu/WTra#warning_for_children_red_white"/>
        <hasSign rdf:resource="https://github.com/danCazacu/WTra#warning_for_traffic_jams_red_white"/>
        <rdfs:comment>Road signs in Ireland do not differ greatly from those used elsewhere in Europe, but there are some differences between those used in the Republic of Ireland and those used in Northern Ireland, including different systems of units used in each jurisdiction.</rdfs:comment>
        <rdfs:seeAlso>https://www.wikiwand.com/en/Italy</rdfs:seeAlso>
    </owl:NamedIndividual>
    


    <!-- https://github.com/danCazacu/WTra#li -->

    <owl:NamedIndividual rdf:about="https://github.com/danCazacu/WTra#li">
        <rdf:type rdf:resource="https://github.com/danCazacu/WTra#Country_Code"/>
    </owl:NamedIndividual>
    


    <!-- https://github.com/danCazacu/WTra#lt -->

    <owl:NamedIndividual rdf:about="https://github.com/danCazacu/WTra#lt">
        <rdf:type rdf:resource="https://github.com/danCazacu/WTra#Country_Code"/>
    </owl:NamedIndividual>
    


    <!-- https://github.com/danCazacu/WTra#mandatory_right -->

    <owl:NamedIndividual rdf:about="https://github.com/danCazacu/WTra#mandatory_right">
        <rdf:type rdf:resource="https://github.com/danCazacu/WTra#Mandatory_Sign"/>
        <applicableTo rdf:resource="https://github.com/danCazacu/WTra#driver"/>
        <hasBackgroundColor rdf:resource="https://github.com/danCazacu/WTra#blue"/>
        <hasBorderColor rdf:resource="https://github.com/danCazacu/WTra#white"/>
        <hasForm rdf:resource="https://github.com/danCazacu/WTra#circle"/>
        <hasImageLink>https://traffic-rules.com/img/europe/ro/signs/mandatory/mandatory-direction-turn-right.png</hasImageLink>
        <hasLegalRegulations>This traffic sign indicates that all drivers must turn right, turning left is not allowed.</hasLegalRegulations>
        <rdfs:comment>This traffic sign indicates that all drivers must turn right, turning left is not allowed.</rdfs:comment>
    </owl:NamedIndividual>
    


    <!-- https://github.com/danCazacu/WTra#mandatory_shared_path_for_pedestrians_and_cyclists -->

    <owl:NamedIndividual rdf:about="https://github.com/danCazacu/WTra#mandatory_shared_path_for_pedestrians_and_cyclists">
        <rdf:type rdf:resource="https://github.com/danCazacu/WTra#Mandatory_Sign"/>
        <applicableTo rdf:resource="https://github.com/danCazacu/WTra#driver"/>
        <applicableTo rdf:resource="https://github.com/danCazacu/WTra#pedestrian"/>
        <hasBackgroundColor rdf:resource="https://github.com/danCazacu/WTra#blue"/>
        <hasBorderColor rdf:resource="https://github.com/danCazacu/WTra#white"/>
        <hasImageLink>https://traffic-rules.com/img/europe/ro/signs/mandatory/mandatory-lane-pedestrian-cyclist.png</hasImageLink>
        <hasLegalRegulations>Way were only pedestrian and cyclists are allowed to go on.</hasLegalRegulations>
        <rdfs:comment>This traffic sign indicates the begin of a shared path for pedestrians and cyclists.</rdfs:comment>
    </owl:NamedIndividual>
    


    <!-- https://github.com/danCazacu/WTra#maximum_speed_limit_red_white -->

    <owl:NamedIndividual rdf:about="https://github.com/danCazacu/WTra#maximum_speed_limit_red_white">
        <rdf:type rdf:resource="https://github.com/danCazacu/WTra#Prohibitory_Sign"/>
        <owl:sameAs rdf:resource="https://github.com/danCazacu/WTra#maximum_speed_limit_red_yellow"/>
        <applicableTo rdf:resource="https://github.com/danCazacu/WTra#driver"/>
        <hasBackgroundColor rdf:resource="https://github.com/danCazacu/WTra#white"/>
        <hasBorderColor rdf:resource="https://github.com/danCazacu/WTra#red"/>
        <hasForm rdf:resource="https://github.com/danCazacu/WTra#circle"/>
        <hasImageLink>https://traffic-rules.com/img/europe/ro/signs/prohibitory/prohibited-action-speed.png</hasImageLink>
        <hasLegalRegulations>The driver is forced to drive with speed below the limit indicating by the traffic sign.</hasLegalRegulations>
        <rdfs:comment>This traffic sign indicates the begin of a zone with a speed limit. On all roads in the zone it’s prohibited to drive faster than indicated.</rdfs:comment>
    </owl:NamedIndividual>
    


    <!-- https://github.com/danCazacu/WTra#maximum_speed_limit_red_yellow -->

    <owl:NamedIndividual rdf:about="https://github.com/danCazacu/WTra#maximum_speed_limit_red_yellow">
        <rdf:type rdf:resource="https://github.com/danCazacu/WTra#Prohibitory_Sign"/>
        <applicableTo rdf:resource="https://github.com/danCazacu/WTra#driver"/>
        <hasBackgroundColor rdf:resource="https://github.com/danCazacu/WTra#yellow"/>
        <hasBorderColor rdf:resource="https://github.com/danCazacu/WTra#red"/>
        <hasForm rdf:resource="https://github.com/danCazacu/WTra#circle"/>
        <hasImageLink>https://traffic-rules.com/img/europe/fi/signs/prohibitory/prohibited-action-speed.png</hasImageLink>
        <hasLegalRegulations>The driver is forced to drive with speed below the limit indicating by the traffic sign.</hasLegalRegulations>
        <rdfs:comment>This traffic sign indicates the begin of a zone with a speed limit. On all roads in the zone it’s prohibited to drive faster than indicated.</rdfs:comment>
    </owl:NamedIndividual>
    


    <!-- https://github.com/danCazacu/WTra#minimum_speed_limit -->

    <owl:NamedIndividual rdf:about="https://github.com/danCazacu/WTra#minimum_speed_limit">
        <rdf:type rdf:resource="https://github.com/danCazacu/WTra#Mandatory_Sign"/>
        <applicableTo rdf:resource="https://github.com/danCazacu/WTra#driver"/>
        <hasBackgroundColor rdf:resource="https://github.com/danCazacu/WTra#blue"/>
        <hasBorderColor rdf:resource="https://github.com/danCazacu/WTra#white"/>
        <hasForm rdf:resource="https://github.com/danCazacu/WTra#circle"/>
        <hasImageLink>https://traffic-rules.com/img/europe/ro/signs/mandatory/mandatory-speed-minimum.png</hasImageLink>
        <hasLegalRegulations>The driver has to drive the card with the minimum speed indicated by the traffic sign.</hasLegalRegulations>
        <rdfs:comment>This traffic sign indicates the begin of a minimum speed. Drive faster than indicated.</rdfs:comment>
    </owl:NamedIndividual>
    


    <!-- https://github.com/danCazacu/WTra#n -->

    <owl:NamedIndividual rdf:about="https://github.com/danCazacu/WTra#n">
        <rdf:type rdf:resource="https://github.com/danCazacu/WTra#Country_Code"/>
    </owl:NamedIndividual>
    


    <!-- https://github.com/danCazacu/WTra#nl -->

    <owl:NamedIndividual rdf:about="https://github.com/danCazacu/WTra#nl">
        <rdf:type rdf:resource="https://github.com/danCazacu/WTra#Country_Code"/>
    </owl:NamedIndividual>
    


    <!-- https://github.com/danCazacu/WTra#no_motor_vehicles_red_white -->

    <owl:NamedIndividual rdf:about="https://github.com/danCazacu/WTra#no_motor_vehicles_red_white">
        <rdf:type rdf:resource="https://github.com/danCazacu/WTra#Prohibitory_Sign"/>
        <owl:sameAs rdf:resource="https://github.com/danCazacu/WTra#no_motor_vehicles_red_yellow"/>
        <applicableTo rdf:resource="https://github.com/danCazacu/WTra#driver"/>
        <hasBackgroundColor rdf:resource="https://github.com/danCazacu/WTra#white"/>
        <hasBorderColor rdf:resource="https://github.com/danCazacu/WTra#red"/>
        <hasForm rdf:resource="https://github.com/danCazacu/WTra#circle"/>
        <hasImageLink>https://traffic-rules.com/img/europe/ro/signs/prohibitory/prohibited-access-motorcycle-car.png</hasImageLink>
        <hasLegalRegulations>The traffic indicates an area were the cars and motorcycle are prohibited.</hasLegalRegulations>
        <rdfs:comment>This traffic sign indicates a place where motorcycles and cars are prohibited. Pedestrians and cyclists are allowed in these places. An example of this would be a market area.</rdfs:comment>
    </owl:NamedIndividual>
    


    <!-- https://github.com/danCazacu/WTra#no_motor_vehicles_red_yellow -->

    <owl:NamedIndividual rdf:about="https://github.com/danCazacu/WTra#no_motor_vehicles_red_yellow">
        <rdf:type rdf:resource="https://github.com/danCazacu/WTra#Prohibitory_Sign"/>
        <applicableTo rdf:resource="https://github.com/danCazacu/WTra#driver"/>
        <hasBackgroundColor rdf:resource="https://github.com/danCazacu/WTra#yellow"/>
        <hasBorderColor rdf:resource="https://github.com/danCazacu/WTra#red"/>
        <hasForm rdf:resource="https://github.com/danCazacu/WTra#circle"/>
        <hasImageLink>https://traffic-rules.com/img/europe/fi/signs/prohibitory/prohibited-access-motorcycle-car.png</hasImageLink>
        <hasLegalRegulations>The traffic indicates an area were the cars and motorcycle are prohibited.</hasLegalRegulations>
        <rdfs:comment>This traffic sign indicates a place where motorcycles and cars are prohibited. Pedestrians and cyclists are allowed in these places. An example of this would be a market area.</rdfs:comment>
    </owl:NamedIndividual>
    


    <!-- https://github.com/danCazacu/WTra#orange -->

    <owl:NamedIndividual rdf:about="https://github.com/danCazacu/WTra#orange">
        <rdf:type rdf:resource="https://github.com/danCazacu/WTra#Color"/>
    </owl:NamedIndividual>
    


    <!-- https://github.com/danCazacu/WTra#other_danger_red_white -->

    <owl:NamedIndividual rdf:about="https://github.com/danCazacu/WTra#other_danger_red_white">
        <rdf:type rdf:resource="https://github.com/danCazacu/WTra#Warning_Sign"/>
        <owl:sameAs rdf:resource="https://github.com/danCazacu/WTra#other_danger_red_yellow"/>
        <applicableTo rdf:resource="https://github.com/danCazacu/WTra#driver"/>
        <hasBackgroundColor rdf:resource="https://github.com/danCazacu/WTra#white"/>
        <hasBorderColor rdf:resource="https://github.com/danCazacu/WTra#red"/>
        <hasForm rdf:resource="https://github.com/danCazacu/WTra#triangle"/>
        <hasImageLink>https://traffic-rules.com/img/europe/ro/signs/warning/warning.png</hasImageLink>
        <hasLegalRegulations>The driver must be very careful as it is a zone were accidents happens offten. It is indicated to reduce the speed.</hasLegalRegulations>
        <rdfs:comment>This traffic sign warns for miscellaneous dangers for which there is no specific traffic sign. For examples: road accidents, flooded roads and roads blocked by fallen trees. It always have a supplementary sign attached that tells drivers of what hazard to expect.</rdfs:comment>
    </owl:NamedIndividual>
    


    <!-- https://github.com/danCazacu/WTra#other_danger_red_yellow -->

    <owl:NamedIndividual rdf:about="https://github.com/danCazacu/WTra#other_danger_red_yellow">
        <rdf:type rdf:resource="https://github.com/danCazacu/WTra#Warning_Sign"/>
        <applicableTo rdf:resource="https://github.com/danCazacu/WTra#driver"/>
        <hasBackgroundColor rdf:resource="https://github.com/danCazacu/WTra#yellow"/>
        <hasBorderColor rdf:resource="https://github.com/danCazacu/WTra#red"/>
        <hasForm rdf:resource="https://github.com/danCazacu/WTra#triangle"/>
        <hasImageLink>https://traffic-rules.com/img/europe/fi/signs/warning/warning.png</hasImageLink>
        <hasLegalRegulations>The driver must be very careful as it is a zone were accidents happens offten. It is indicated to reduce the speed.</hasLegalRegulations>
        <rdfs:comment>This traffic sign warns for miscellaneous dangers for which there is no specific traffic sign. For examples: road accidents, flooded roads and roads blocked by fallen trees. It always have a supplementary sign attached that tells drivers of what hazard to expect.</rdfs:comment>
    </owl:NamedIndividual>
    


    <!-- https://github.com/danCazacu/WTra#p -->

    <owl:NamedIndividual rdf:about="https://github.com/danCazacu/WTra#p">
        <rdf:type rdf:resource="https://github.com/danCazacu/WTra#Country_Code"/>
    </owl:NamedIndividual>
    


    <!-- https://github.com/danCazacu/WTra#pedestrian -->

    <owl:NamedIndividual rdf:about="https://github.com/danCazacu/WTra#pedestrian">
        <rdf:type rdf:resource="https://github.com/danCazacu/WTra#Person"/>
    </owl:NamedIndividual>
    


    <!-- https://github.com/danCazacu/WTra#pedestrians_prohibited_red_white -->

    <owl:NamedIndividual rdf:about="https://github.com/danCazacu/WTra#pedestrians_prohibited_red_white">
        <rdf:type rdf:resource="https://github.com/danCazacu/WTra#Prohibitory_Sign"/>
        <owl:sameAs rdf:resource="https://github.com/danCazacu/WTra#pedestrians_prohibited_red_yellow"/>
        <applicableTo rdf:resource="https://github.com/danCazacu/WTra#driver"/>
        <applicableTo rdf:resource="https://github.com/danCazacu/WTra#pedestrian"/>
        <hasBackgroundColor rdf:resource="https://github.com/danCazacu/WTra#white"/>
        <hasBorderColor rdf:resource="https://github.com/danCazacu/WTra#red"/>
        <hasForm rdf:resource="https://github.com/danCazacu/WTra#circle"/>
        <hasImageLink>https://traffic-rules.com/img/europe/ro/signs/prohibitory/prohibited-access-pedestrian.png</hasImageLink>
        <hasLegalRegulations>The sign indicates an area were the pedestrian can not enter.</hasLegalRegulations>
        <rdfs:comment>This traffic sign indicates a place where pedestrians are prohibited, such as certain bridges or flyovers where separate provisions have been made for pedestrians.</rdfs:comment>
    </owl:NamedIndividual>
    


    <!-- https://github.com/danCazacu/WTra#pedestrians_prohibited_red_yellow -->

    <owl:NamedIndividual rdf:about="https://github.com/danCazacu/WTra#pedestrians_prohibited_red_yellow">
        <rdf:type rdf:resource="https://github.com/danCazacu/WTra#Prohibitory_Sign"/>
        <applicableTo rdf:resource="https://github.com/danCazacu/WTra#driver"/>
        <applicableTo rdf:resource="https://github.com/danCazacu/WTra#pedestrian"/>
        <hasBackgroundColor rdf:resource="https://github.com/danCazacu/WTra#yellow"/>
        <hasBorderColor rdf:resource="https://github.com/danCazacu/WTra#red"/>
        <hasForm rdf:resource="https://github.com/danCazacu/WTra#circle"/>
        <hasImageLink>https://traffic-rules.com/img/europe/fi/signs/prohibitory/prohibited-access-pedestrian.png</hasImageLink>
        <hasLegalRegulations>The sign indicates an area were the pedestrian can not enter.</hasLegalRegulations>
        <rdfs:comment>This traffic sign indicates a place where pedestrians are prohibited, such as certain bridges or flyovers where separate provisions have been made for pedestrians.</rdfs:comment>
    </owl:NamedIndividual>
    


    <!-- https://github.com/danCazacu/WTra#pink -->

    <owl:NamedIndividual rdf:about="https://github.com/danCazacu/WTra#pink">
        <rdf:type rdf:resource="https://github.com/danCazacu/WTra#Color"/>
    </owl:NamedIndividual>
    


    <!-- https://github.com/danCazacu/WTra#pl -->

    <owl:NamedIndividual rdf:about="https://github.com/danCazacu/WTra#pl">
        <rdf:type rdf:resource="https://github.com/danCazacu/WTra#Country_Code"/>
    </owl:NamedIndividual>
    


    <!-- https://github.com/danCazacu/WTra#red -->

    <owl:NamedIndividual rdf:about="https://github.com/danCazacu/WTra#red">
        <rdf:type rdf:resource="https://github.com/danCazacu/WTra#Color"/>
        <hasForm rdf:resource="https://github.com/danCazacu/WTra#circle"/>
    </owl:NamedIndividual>
    


    <!-- https://github.com/danCazacu/WTra#red_white -->

    <owl:NamedIndividual rdf:about="https://github.com/danCazacu/WTra#red_white">
        <hasBackgroundColor rdf:resource="https://github.com/danCazacu/WTra#white"/>
        <hasBorderColor rdf:resource="https://github.com/danCazacu/WTra#red"/>
        <hasImageLink>https://traffic-rules.com/img/europe/ro/signs/warning/warning-crossroad-give-way.png</hasImageLink>
    </owl:NamedIndividual>
    


    <!-- https://github.com/danCazacu/WTra#red_yellow -->

    <owl:NamedIndividual rdf:about="https://github.com/danCazacu/WTra#red_yellow">
        <hasBackgroundColor rdf:resource="https://github.com/danCazacu/WTra#yellow"/>
        <hasBorderColor rdf:resource="https://github.com/danCazacu/WTra#red"/>
    </owl:NamedIndividual>
    


    <!-- https://github.com/danCazacu/WTra#ro -->

    <owl:NamedIndividual rdf:about="https://github.com/danCazacu/WTra#ro">
        <rdf:type rdf:resource="https://github.com/danCazacu/WTra#Country_Code"/>
        <isCountry rdf:resource="https://github.com/danCazacu/WTra#romania"/>
    </owl:NamedIndividual>
    


    <!-- https://github.com/danCazacu/WTra#romania -->

    <owl:NamedIndividual rdf:about="https://github.com/danCazacu/WTra#romania">
        <rdf:type rdf:resource="https://github.com/danCazacu/WTra#Country"/>
        <hasCode rdf:resource="https://github.com/danCazacu/WTra#ro"/>
        <hasSign rdf:resource="https://github.com/danCazacu/WTra#begin_of_a_priority_road"/>
        <hasSign rdf:resource="https://github.com/danCazacu/WTra#crossing_for_pedestrians"/>
        <hasSign rdf:resource="https://github.com/danCazacu/WTra#end_of_the_priority_road_one_line"/>
        <hasSign rdf:resource="https://github.com/danCazacu/WTra#end_of_the_speed_limit_one_line"/>
        <hasSign rdf:resource="https://github.com/danCazacu/WTra#give_way_to_all_drivers_red_white"/>
        <hasSign rdf:resource="https://github.com/danCazacu/WTra#mandatory_right"/>
        <hasSign rdf:resource="https://github.com/danCazacu/WTra#mandatory_shared_path_for_pedestrians_and_cyclists"/>
        <hasSign rdf:resource="https://github.com/danCazacu/WTra#maximum_speed_limit_red_white"/>
        <hasSign rdf:resource="https://github.com/danCazacu/WTra#minimum_speed_limit"/>
        <hasSign rdf:resource="https://github.com/danCazacu/WTra#no_motor_vehicles_red_white"/>
        <hasSign rdf:resource="https://github.com/danCazacu/WTra#other_danger_red_white"/>
        <hasSign rdf:resource="https://github.com/danCazacu/WTra#pedestrians_prohibited_red_white"/>
        <hasSign rdf:resource="https://github.com/danCazacu/WTra#stop_and_give_way_to_all_drivers"/>
        <hasSign rdf:resource="https://github.com/danCazacu/WTra#turning_left_prohibited_red_white"/>
        <hasSign rdf:resource="https://github.com/danCazacu/WTra#turning_right_mandatory"/>
        <hasSign rdf:resource="https://github.com/danCazacu/WTra#turning_right_prohibited_red_white"/>
        <hasSign rdf:resource="https://github.com/danCazacu/WTra#warning_for_a_crossing_for_pedestrians_red_white"/>
        <hasSign rdf:resource="https://github.com/danCazacu/WTra#warning_for_a_traffic_light_red_white"/>
        <hasSign rdf:resource="https://github.com/danCazacu/WTra#warning_for_children_red_white"/>
        <hasSign rdf:resource="https://github.com/danCazacu/WTra#warning_for_traffic_jams_red_white"/>
        <rdfs:seeAlso>https://www.wikiwand.com/en/Romania</rdfs:seeAlso>
    </owl:NamedIndividual>
    


    <!-- https://github.com/danCazacu/WTra#s -->

    <owl:NamedIndividual rdf:about="https://github.com/danCazacu/WTra#s">
        <rdf:type rdf:resource="https://github.com/danCazacu/WTra#Country_Code"/>
    </owl:NamedIndividual>
    


    <!-- https://github.com/danCazacu/WTra#sk -->

    <owl:NamedIndividual rdf:about="https://github.com/danCazacu/WTra#sk">
        <rdf:type rdf:resource="https://github.com/danCazacu/WTra#Country_Code"/>
    </owl:NamedIndividual>
    


    <!-- https://github.com/danCazacu/WTra#square -->

    <owl:NamedIndividual rdf:about="https://github.com/danCazacu/WTra#square">
        <rdf:type rdf:resource="https://github.com/danCazacu/WTra#Shape"/>
    </owl:NamedIndividual>
    


    <!-- https://github.com/danCazacu/WTra#stop_and_give_way_to_all_drivers -->

    <owl:NamedIndividual rdf:about="https://github.com/danCazacu/WTra#stop_and_give_way_to_all_drivers">
        <rdf:type rdf:resource="https://github.com/danCazacu/WTra#Priority_Sign"/>
        <rdf:type rdf:resource="https://github.com/danCazacu/WTra#Warning_Sign"/>
        <owl:sameAs rdf:resource="https://github.com/danCazacu/WTra#stop_and_give_way_to_all_drivers_triangle"/>
        <applicableTo rdf:resource="https://github.com/danCazacu/WTra#driver"/>
        <hasBackgroundColor rdf:resource="https://github.com/danCazacu/WTra#red"/>
        <hasBorderColor rdf:resource="https://github.com/danCazacu/WTra#white"/>
        <hasForm rdf:resource="https://github.com/danCazacu/WTra#hexagon"/>
        <hasImageLink>https://traffic-rules.com/img/europe/ro/signs/warning/warning-crossroad-stop.png</hasImageLink>
        <hasLegalRegulations>This traffic sign means that the driver is not allowed to enter the crossroad unless the road is clear. The driver is forced to stop.</hasLegalRegulations>
        <rdfs:comment>This traffic sign warns for a crossroad where visibility is poor or unsafe for drivers to enter the crossroad without stopping. It instructs drivers to bring their vehicles to a complete stop and not proceed until it is safe to do so.</rdfs:comment>
    </owl:NamedIndividual>
    


    <!-- https://github.com/danCazacu/WTra#stop_and_give_way_to_all_drivers_triangle -->

    <owl:NamedIndividual rdf:about="https://github.com/danCazacu/WTra#stop_and_give_way_to_all_drivers_triangle">
        <rdf:type rdf:resource="https://github.com/danCazacu/WTra#Priority_Sign"/>
        <rdf:type rdf:resource="https://github.com/danCazacu/WTra#Warning_Sign"/>
        <applicableTo rdf:resource="https://github.com/danCazacu/WTra#driver"/>
        <hasBackgroundColor rdf:resource="https://github.com/danCazacu/WTra#white"/>
        <hasBorderColor rdf:resource="https://github.com/danCazacu/WTra#red"/>
        <hasForm rdf:resource="https://github.com/danCazacu/WTra#triangle"/>
        <hasLegalRegulations>This traffic sign means that the driver is not allowed to enter the crossroad unless the road is clear. The driver is forced to stop.</hasLegalRegulations>
        <rdfs:comment>This traffic sign warns for a crossroad where visibility is poor or unsafe for drivers to enter the crossroad without stopping. It instructs drivers to bring their vehicles to a complete stop and not proceed until it is safe to do so.</rdfs:comment>
    </owl:NamedIndividual>
    


    <!-- https://github.com/danCazacu/WTra#triangle -->

    <owl:NamedIndividual rdf:about="https://github.com/danCazacu/WTra#triangle">
        <rdf:type rdf:resource="https://github.com/danCazacu/WTra#Shape"/>
    </owl:NamedIndividual>
    


    <!-- https://github.com/danCazacu/WTra#turning_left_prohibited_red_white -->

    <owl:NamedIndividual rdf:about="https://github.com/danCazacu/WTra#turning_left_prohibited_red_white">
        <rdf:type rdf:resource="https://github.com/danCazacu/WTra#Prohibitory_Sign"/>
        <owl:sameAs rdf:resource="https://github.com/danCazacu/WTra#turning_left_prohibited_red_yellow"/>
        <applicableTo rdf:resource="https://github.com/danCazacu/WTra#driver"/>
        <hasBackgroundColor rdf:resource="https://github.com/danCazacu/WTra#white"/>
        <hasBorderColor rdf:resource="https://github.com/danCazacu/WTra#red"/>
        <hasForm rdf:resource="https://github.com/danCazacu/WTra#circle"/>
        <hasImageLink>https://traffic-rules.com/img/europe/ro/signs/prohibitory/prohibited-action-turn-left.png</hasImageLink>
        <hasLegalRegulations>The sign indicates a place were the driver can not turn left in the first intersection.</hasLegalRegulations>
        <rdfs:comment>This traffic sign indicates a place where turning left into a side road is prohibited. This normally occurs where either the side road is one way in the opposite direction or vehicles waiting to turn left would cause traffic congestion.</rdfs:comment>
    </owl:NamedIndividual>
    


    <!-- https://github.com/danCazacu/WTra#turning_left_prohibited_red_yellow -->

    <owl:NamedIndividual rdf:about="https://github.com/danCazacu/WTra#turning_left_prohibited_red_yellow">
        <rdf:type rdf:resource="https://github.com/danCazacu/WTra#Prohibitory_Sign"/>
        <applicableTo rdf:resource="https://github.com/danCazacu/WTra#driver"/>
        <hasBackgroundColor rdf:resource="https://github.com/danCazacu/WTra#yellow"/>
        <hasBorderColor rdf:resource="https://github.com/danCazacu/WTra#red"/>
        <hasForm rdf:resource="https://github.com/danCazacu/WTra#circle"/>
        <hasImageLink>https://traffic-rules.com/img/europe/fi/signs/prohibitory/prohibited-action-turn-left.png</hasImageLink>
        <hasLegalRegulations>The sign indicates a place were the driver can not turn left in the first intersection.</hasLegalRegulations>
        <rdfs:comment>This traffic sign indicates a place where turning left into a side road is prohibited. This normally occurs where either the side road is one way in the opposite direction or vehicles waiting to turn left would cause traffic congestion.</rdfs:comment>
    </owl:NamedIndividual>
    


    <!-- https://github.com/danCazacu/WTra#turning_right_mandatory -->

    <owl:NamedIndividual rdf:about="https://github.com/danCazacu/WTra#turning_right_mandatory">
        <rdf:type rdf:resource="https://github.com/danCazacu/WTra#Mandatory_Sign"/>
        <applicableTo rdf:resource="https://github.com/danCazacu/WTra#driver"/>
        <hasBackgroundColor rdf:resource="https://github.com/danCazacu/WTra#blue"/>
        <hasBorderColor rdf:resource="https://github.com/danCazacu/WTra#white"/>
        <hasForm rdf:resource="https://github.com/danCazacu/WTra#circle"/>
        <hasImageLink>https://traffic-rules.com/img/europe/ro/signs/mandatory/mandatory-direction-ahead-turn-right.png</hasImageLink>
        <hasLegalRegulations>This traffic sign indicates that all drivers must turn right, other directions are not allowed.</hasLegalRegulations>
        <rdfs:comment>This traffic sign indicates that all drivers must turn right, other directions are not allowed.</rdfs:comment>
    </owl:NamedIndividual>
    


    <!-- https://github.com/danCazacu/WTra#turning_right_prohibited_red_white -->

    <owl:NamedIndividual rdf:about="https://github.com/danCazacu/WTra#turning_right_prohibited_red_white">
        <rdf:type rdf:resource="https://github.com/danCazacu/WTra#Prohibitory_Sign"/>
        <owl:sameAs rdf:resource="https://github.com/danCazacu/WTra#turning_right_prohibited_red_yellow"/>
        <applicableTo rdf:resource="https://github.com/danCazacu/WTra#driver"/>
        <hasBackgroundColor rdf:resource="https://github.com/danCazacu/WTra#white"/>
        <hasBorderColor rdf:resource="https://github.com/danCazacu/WTra#red"/>
        <hasForm rdf:resource="https://github.com/danCazacu/WTra#circle"/>
        <hasImageLink>https://traffic-rules.com/img/europe/ro/signs/prohibitory/prohibited-action-turn-right.png</hasImageLink>
        <hasLegalRegulations>The sign indicates a place were the driver can not turn right in the first intersection.</hasLegalRegulations>
        <rdfs:comment>This traffic sign indicates a place where turning right into a side road is prohibited. This normally occurs where either the side road is one way in the opposite direction or vehicles waiting to turn right would cause traffic congestion.</rdfs:comment>
    </owl:NamedIndividual>
    


    <!-- https://github.com/danCazacu/WTra#turning_right_prohibited_red_yellow -->

    <owl:NamedIndividual rdf:about="https://github.com/danCazacu/WTra#turning_right_prohibited_red_yellow">
        <rdf:type rdf:resource="https://github.com/danCazacu/WTra#Prohibitory_Sign"/>
        <applicableTo rdf:resource="https://github.com/danCazacu/WTra#driver"/>
        <hasBackgroundColor rdf:resource="https://github.com/danCazacu/WTra#yellow"/>
        <hasBorderColor rdf:resource="https://github.com/danCazacu/WTra#red"/>
        <hasForm rdf:resource="https://github.com/danCazacu/WTra#circle"/>
        <hasImageLink>https://traffic-rules.com/img/europe/fi/signs/prohibitory/prohibited-action-turn-right.png</hasImageLink>
        <hasLegalRegulations>The sign indicates a place were the driver can not turn right in the first intersection.</hasLegalRegulations>
        <rdfs:comment>This traffic sign indicates a place where turning right into a side road is prohibited. This normally occurs where either the side road is one way in the opposite direction or vehicles waiting to turn right would cause traffic congestion.</rdfs:comment>
    </owl:NamedIndividual>
    


    <!-- https://github.com/danCazacu/WTra#united_kindom -->

    <owl:NamedIndividual rdf:about="https://github.com/danCazacu/WTra#united_kindom">
        <rdf:type rdf:resource="https://github.com/danCazacu/WTra#Country"/>
        <hasCode rdf:resource="https://github.com/danCazacu/WTra#gb"/>
        <hasNotSign rdf:resource="https://github.com/danCazacu/WTra#begin_of_a_priority_road"/>
        <hasNotSign rdf:resource="https://github.com/danCazacu/WTra#crossing_for_pedestrians"/>
        <hasNotSign rdf:resource="https://github.com/danCazacu/WTra#end_of_the_priority_road_one_3_lines"/>
        <hasNotSign rdf:resource="https://github.com/danCazacu/WTra#end_of_the_priority_road_one_line"/>
        <hasNotSign rdf:resource="https://github.com/danCazacu/WTra#other_danger_red_white"/>
        <hasNotSign rdf:resource="https://github.com/danCazacu/WTra#other_danger_red_yellow"/>
        <hasSign rdf:resource="https://github.com/danCazacu/WTra#end_of_the_speed_limit_one_line"/>
        <hasSign rdf:resource="https://github.com/danCazacu/WTra#give_way_to_all_drivers_red_white"/>
        <hasSign rdf:resource="https://github.com/danCazacu/WTra#mandatory_right"/>
        <hasSign rdf:resource="https://github.com/danCazacu/WTra#mandatory_shared_path_for_pedestrians_and_cyclists"/>
        <hasSign rdf:resource="https://github.com/danCazacu/WTra#maximum_speed_limit_red_white"/>
        <hasSign rdf:resource="https://github.com/danCazacu/WTra#minimum_speed_limit"/>
        <hasSign rdf:resource="https://github.com/danCazacu/WTra#no_motor_vehicles_red_white"/>
        <hasSign rdf:resource="https://github.com/danCazacu/WTra#pedestrians_prohibited_red_white"/>
        <hasSign rdf:resource="https://github.com/danCazacu/WTra#stop_and_give_way_to_all_drivers"/>
        <hasSign rdf:resource="https://github.com/danCazacu/WTra#turning_left_prohibited_red_white"/>
        <hasSign rdf:resource="https://github.com/danCazacu/WTra#turning_right_mandatory"/>
        <hasSign rdf:resource="https://github.com/danCazacu/WTra#turning_right_prohibited_red_white"/>
        <hasSign rdf:resource="https://github.com/danCazacu/WTra#warning_for_a_crossing_for_pedestrians_red_white"/>
        <hasSign rdf:resource="https://github.com/danCazacu/WTra#warning_for_a_traffic_light_red_white"/>
        <hasSign rdf:resource="https://github.com/danCazacu/WTra#warning_for_children_red_white"/>
        <hasSign rdf:resource="https://github.com/danCazacu/WTra#warning_for_traffic_jams_red_white"/>
        <rdfs:comment>Road signs in the United Kingdom conform broadly to European design norms, though a number of signs are unique: direction signs omit European route numbers and road signs generally use the Imperial System of units (miles and yards), unlike the rest of Europe (km and m). A range of signs are used on British roads such as destination signposts, signs warning of possible hazards ahead, and regulatory signs instructing road users to perform specific actions.</rdfs:comment>
    </owl:NamedIndividual>
    


    <!-- https://github.com/danCazacu/WTra#warning_for_a_crossing_for_pedestrians_red_white -->

    <owl:NamedIndividual rdf:about="https://github.com/danCazacu/WTra#warning_for_a_crossing_for_pedestrians_red_white">
        <rdf:type rdf:resource="https://github.com/danCazacu/WTra#Warning_Sign"/>
        <owl:sameAs rdf:resource="https://github.com/danCazacu/WTra#warning_for_a_crossing_for_pedestrians_red_yellow"/>
        <applicableTo rdf:resource="https://github.com/danCazacu/WTra#driver"/>
        <hasBackgroundColor rdf:resource="https://github.com/danCazacu/WTra#white"/>
        <hasBorderColor rdf:resource="https://github.com/danCazacu/WTra#red"/>
        <hasForm rdf:resource="https://github.com/danCazacu/WTra#triangle"/>
        <hasImageLink>https://traffic-rules.com/img/europe/ro/signs/warning/warning-pedestrian-crossing.png</hasImageLink>
        <hasLegalRegulations>The drivers have to reduce the speed and prepare to give priority to pedestrian on the zebra crossing.</hasLegalRegulations>
        <rdfs:comment>This traffic sign warns for a pedestrian crossing. The traffic sign is used at crossings that are difficult to see or on roads with a high speed. Drivers must give priority to pedestrians on the zebra crossing.</rdfs:comment>
    </owl:NamedIndividual>
    


    <!-- https://github.com/danCazacu/WTra#warning_for_a_crossing_for_pedestrians_red_yellow -->

    <owl:NamedIndividual rdf:about="https://github.com/danCazacu/WTra#warning_for_a_crossing_for_pedestrians_red_yellow">
        <rdf:type rdf:resource="https://github.com/danCazacu/WTra#Warning_Sign"/>
        <applicableTo rdf:resource="https://github.com/danCazacu/WTra#driver"/>
        <hasBackgroundColor rdf:resource="https://github.com/danCazacu/WTra#yellow"/>
        <hasBorderColor rdf:resource="https://github.com/danCazacu/WTra#red"/>
        <hasForm rdf:resource="https://github.com/danCazacu/WTra#triangle"/>
        <hasImageLink>https://traffic-rules.com/img/europe/fi/signs/warning/warning-pedestrian-crossing.png</hasImageLink>
        <hasLegalRegulations>The drivers have to reduce the speed and prepare to give priority to pedestrian on the zebra crossing.</hasLegalRegulations>
        <rdfs:comment>This traffic sign warns for a pedestrian crossing. The traffic sign is used at crossings that are difficult to see or on roads with a high speed. Drivers must give priority to pedestrians on the zebra crossing.</rdfs:comment>
    </owl:NamedIndividual>
    


    <!-- https://github.com/danCazacu/WTra#warning_for_a_traffic_light_diamond -->

    <owl:NamedIndividual rdf:about="https://github.com/danCazacu/WTra#warning_for_a_traffic_light_diamond">
        <rdf:type rdf:resource="https://github.com/danCazacu/WTra#Warning_Sign"/>
        <owl:sameAs rdf:resource="https://github.com/danCazacu/WTra#warning_for_a_traffic_light_red_white"/>
        <owl:sameAs rdf:resource="https://github.com/danCazacu/WTra#warning_for_a_traffic_light_red_yellow"/>
        <applicableTo rdf:resource="https://github.com/danCazacu/WTra#driver"/>
        <hasBackgroundColor rdf:resource="https://github.com/danCazacu/WTra#yellow"/>
        <hasBorderColor rdf:resource="https://github.com/danCazacu/WTra#black"/>
        <hasForm rdf:resource="https://github.com/danCazacu/WTra#diamond"/>
        <hasImageLink>https://traffic-rules.com/img/europe/ie/signs/warning/warning-traffic-lights.png</hasImageLink>
        <hasLegalRegulations>The driver must be careful. The sign indicates that follows a intersection directed by traffic lights.</hasLegalRegulations>
    </owl:NamedIndividual>
    


    <!-- https://github.com/danCazacu/WTra#warning_for_a_traffic_light_red_white -->

    <owl:NamedIndividual rdf:about="https://github.com/danCazacu/WTra#warning_for_a_traffic_light_red_white">
        <rdf:type rdf:resource="https://github.com/danCazacu/WTra#Warning_Sign"/>
        <owl:sameAs rdf:resource="https://github.com/danCazacu/WTra#warning_for_a_traffic_light_red_yellow"/>
        <applicableTo rdf:resource="https://github.com/danCazacu/WTra#driver"/>
        <hasBackgroundColor rdf:resource="https://github.com/danCazacu/WTra#white"/>
        <hasBorderColor rdf:resource="https://github.com/danCazacu/WTra#red"/>
        <hasForm rdf:resource="https://github.com/danCazacu/WTra#triangle"/>
        <hasImageLink>https://traffic-rules.com/img/europe/ro/signs/warning/warning-traffic-lights.png</hasImageLink>
        <hasLegalRegulations>The driver must be careful. The sign indicates that follows a intersection directed by traffic lights.</hasLegalRegulations>
        <rdfs:comment>This traffic sign warns that there are traffic lights ahead. Watch out for the traffic light and make sure you can stop on time.</rdfs:comment>
    </owl:NamedIndividual>
    


    <!-- https://github.com/danCazacu/WTra#warning_for_a_traffic_light_red_yellow -->

    <owl:NamedIndividual rdf:about="https://github.com/danCazacu/WTra#warning_for_a_traffic_light_red_yellow">
        <rdf:type rdf:resource="https://github.com/danCazacu/WTra#Warning_Sign"/>
        <applicableTo rdf:resource="https://github.com/danCazacu/WTra#driver"/>
        <hasBackgroundColor rdf:resource="https://github.com/danCazacu/WTra#yellow"/>
        <hasBorderColor rdf:resource="https://github.com/danCazacu/WTra#red"/>
        <hasForm rdf:resource="https://github.com/danCazacu/WTra#triangle"/>
        <hasImageLink>https://traffic-rules.com/img/europe/ro/signs/warning/warning-traffic-lights.png</hasImageLink>
        <hasLegalRegulations>The driver must be careful. The sign indicates that follows a intersection directed by traffic lights.</hasLegalRegulations>
        <rdfs:comment>This traffic sign warns that there are traffic lights ahead. Watch out for the traffic light and make sure you can stop on time.</rdfs:comment>
    </owl:NamedIndividual>
    


    <!-- https://github.com/danCazacu/WTra#warning_for_children_red_white -->

    <owl:NamedIndividual rdf:about="https://github.com/danCazacu/WTra#warning_for_children_red_white">
        <rdf:type rdf:resource="https://github.com/danCazacu/WTra#Warning_Sign"/>
        <owl:sameAs rdf:resource="https://github.com/danCazacu/WTra#warning_for_children_red_yellow"/>
        <applicableTo rdf:resource="https://github.com/danCazacu/WTra#driver"/>
        <hasBackgroundColor rdf:resource="https://github.com/danCazacu/WTra#white"/>
        <hasBorderColor rdf:resource="https://github.com/danCazacu/WTra#red"/>
        <hasForm rdf:resource="https://github.com/danCazacu/WTra#triangle"/>
        <hasImageLink>https://traffic-rules.com/img/europe/ro/signs/warning/warning-children.png</hasImageLink>
        <hasLegalRegulations>The drivers have to reduce the speed and drive very carefully as it is a zone were children can pass the road.</hasLegalRegulations>
        <rdfs:comment>This traffic sign warns that this road is often used by children. Slow down and watch out for children playing. The traffic sign is placed near schools and playgrounds.</rdfs:comment>
    </owl:NamedIndividual>
    


    <!-- https://github.com/danCazacu/WTra#warning_for_children_red_yellow -->

    <owl:NamedIndividual rdf:about="https://github.com/danCazacu/WTra#warning_for_children_red_yellow">
        <rdf:type rdf:resource="https://github.com/danCazacu/WTra#Warning_Sign"/>
        <applicableTo rdf:resource="https://github.com/danCazacu/WTra#driver"/>
        <hasBackgroundColor rdf:resource="https://github.com/danCazacu/WTra#yellow"/>
        <hasBorderColor rdf:resource="https://github.com/danCazacu/WTra#red"/>
        <hasForm rdf:resource="https://github.com/danCazacu/WTra#triangle"/>
        <hasImageLink>https://traffic-rules.com/img/europe/fi/signs/warning/warning-children.png</hasImageLink>
        <hasLegalRegulations>The drivers have to reduce the speed and drive very carefully as it is a zone were children can pass the road.</hasLegalRegulations>
        <rdfs:comment>This traffic sign warns that this road is often used by children. Slow down and watch out for children playing. The traffic sign is placed near schools and playgrounds.</rdfs:comment>
    </owl:NamedIndividual>
    


    <!-- https://github.com/danCazacu/WTra#warning_for_falling_materials -->

    <owl:NamedIndividual rdf:about="https://github.com/danCazacu/WTra#warning_for_falling_materials">
        <rdf:type rdf:resource="https://github.com/danCazacu/WTra#Safety_Sign"/>
        <hasImageLink>https://traffic-rules.com/img/international/safety-signs/warning-falling-parts.png</hasImageLink>
    </owl:NamedIndividual>
    


    <!-- https://github.com/danCazacu/WTra#warning_for_falling_off -->

    <owl:NamedIndividual rdf:about="https://github.com/danCazacu/WTra#warning_for_falling_off">
        <rdf:type rdf:resource="https://github.com/danCazacu/WTra#Safety_Sign"/>
        <hasImageLink>https://traffic-rules.com/img/international/safety-signs/warning-falling.png</hasImageLink>
    </owl:NamedIndividual>
    


    <!-- https://github.com/danCazacu/WTra#warning_for_flammable_materials -->

    <owl:NamedIndividual rdf:about="https://github.com/danCazacu/WTra#warning_for_flammable_materials">
        <rdf:type rdf:resource="https://github.com/danCazacu/WTra#Safety_Sign"/>
        <hasImageLink>https://traffic-rules.com/img/international/safety-signs/warning-flammable.png</hasImageLink>
    </owl:NamedIndividual>
    


    <!-- https://github.com/danCazacu/WTra#warning_for_toxic_substances -->

    <owl:NamedIndividual rdf:about="https://github.com/danCazacu/WTra#warning_for_toxic_substances">
        <rdf:type rdf:resource="https://github.com/danCazacu/WTra#Safety_Sign"/>
        <hasImageLink>https://traffic-rules.com/img/international/safety-signs/warning-poisonous.png</hasImageLink>
    </owl:NamedIndividual>
    


    <!-- https://github.com/danCazacu/WTra#warning_for_traffic_jams_red_black -->

    <owl:NamedIndividual rdf:about="https://github.com/danCazacu/WTra#warning_for_traffic_jams_red_black">
        <rdf:type rdf:resource="https://github.com/danCazacu/WTra#Warning_Sign"/>
        <owl:sameAs rdf:resource="https://github.com/danCazacu/WTra#warning_for_traffic_jams_red_white"/>
        <applicableTo rdf:resource="https://github.com/danCazacu/WTra#driver"/>
        <hasBackgroundColor rdf:resource="https://github.com/danCazacu/WTra#black"/>
        <hasBorderColor rdf:resource="https://github.com/danCazacu/WTra#red"/>
        <hasForm rdf:resource="https://github.com/danCazacu/WTra#triangle"/>
        <hasImageLink>https://traffic-rules.com/img/europe/fi/signs/warning/warning-traffic-que.png</hasImageLink>
        <hasLegalRegulations>The drivers are attentioned to drive carrefully and to have patient as it follows a zone were usually is very crowded.</hasLegalRegulations>
        <rdfs:comment>This traffic sign warns that there is an increased chance of traffic jams. Keep a safe distance from the vehicle in front of you, because the traffic can suddenly slow down.</rdfs:comment>
    </owl:NamedIndividual>
    


    <!-- https://github.com/danCazacu/WTra#warning_for_traffic_jams_red_white -->

    <owl:NamedIndividual rdf:about="https://github.com/danCazacu/WTra#warning_for_traffic_jams_red_white">
        <rdf:type rdf:resource="https://github.com/danCazacu/WTra#Warning_Sign"/>
        <owl:sameAs rdf:resource="https://github.com/danCazacu/WTra#warning_for_traffic_jams_red_yellow"/>
        <applicableTo rdf:resource="https://github.com/danCazacu/WTra#driver"/>
        <hasBackgroundColor rdf:resource="https://github.com/danCazacu/WTra#white"/>
        <hasBorderColor rdf:resource="https://github.com/danCazacu/WTra#red"/>
        <hasForm rdf:resource="https://github.com/danCazacu/WTra#triangle"/>
        <hasImageLink>https://traffic-rules.com/img/europe/ro/signs/warning/warning-traffic-que.png</hasImageLink>
        <hasLegalRegulations>The drivers are attentioned to drive carrefully and to have patient as it follows a zone were usually is very crowded</hasLegalRegulations>
        <rdfs:comment>This traffic sign warns that there is an increased chance of traffic jams. Keep a safe distance from the vehicle in front of you, because the traffic can suddenly slow down.</rdfs:comment>
    </owl:NamedIndividual>
    


    <!-- https://github.com/danCazacu/WTra#warning_for_traffic_jams_red_yellow -->

    <owl:NamedIndividual rdf:about="https://github.com/danCazacu/WTra#warning_for_traffic_jams_red_yellow">
        <rdf:type rdf:resource="https://github.com/danCazacu/WTra#Warning_Sign"/>
        <applicableTo rdf:resource="https://github.com/danCazacu/WTra#driver"/>
        <hasBackgroundColor rdf:resource="https://github.com/danCazacu/WTra#yellow"/>
        <hasBorderColor rdf:resource="https://github.com/danCazacu/WTra#red"/>
        <hasForm rdf:resource="https://github.com/danCazacu/WTra#triangle"/>
        <hasImageLink>https://traffic-rules.com/img/europe/gr/signs/warning/warning-traffic-que.png</hasImageLink>
        <hasLegalRegulations>The drivers are attentioned to drive carrefully and to have patient as it follows a zone were usually is very crowded</hasLegalRegulations>
        <rdfs:comment>This traffic sign warns that there is an increased chance of traffic jams. Keep a safe distance from the vehicle in front of you, because the traffic can suddenly slow down.</rdfs:comment>
    </owl:NamedIndividual>
    


    <!-- https://github.com/danCazacu/WTra#white -->

    <owl:NamedIndividual rdf:about="https://github.com/danCazacu/WTra#white">
        <rdf:type rdf:resource="https://github.com/danCazacu/WTra#Color"/>
    </owl:NamedIndividual>
    


    <!-- https://github.com/danCazacu/WTra#yellow -->

    <owl:NamedIndividual rdf:about="https://github.com/danCazacu/WTra#yellow">
        <rdf:type rdf:resource="https://github.com/danCazacu/WTra#Color"/>
    </owl:NamedIndividual>
    


    <!-- 
    ///////////////////////////////////////////////////////////////////////////////////////
    //
    // General axioms
    //
    ///////////////////////////////////////////////////////////////////////////////////////
     -->

    <rdf:Description>
        <rdf:type rdf:resource="http://www.w3.org/2002/07/owl#AllDisjointClasses"/>
        <owl:members rdf:parseType="Collection">
            <rdf:Description rdf:about="https://github.com/danCazacu/WTra#Information_Sign"/>
            <rdf:Description rdf:about="https://github.com/danCazacu/WTra#Mandatory_Sign"/>
            <rdf:Description rdf:about="https://github.com/danCazacu/WTra#Priority_Sign"/>
            <rdf:Description rdf:about="https://github.com/danCazacu/WTra#Prohibitory_Sign"/>
            <rdf:Description rdf:about="https://github.com/danCazacu/WTra#Warning_Sign"/>
        </owl:members>
    </rdf:Description>
</rdf:RDF>



<!-- Generated by the OWL API (version 4.5.9.2019-02-01T07:24:44Z) https://github.com/owlcs/owlapi -->

